progs/threads.h
@@ -19,6 +19,8 @@ void makelock2(void *lock); //for recursive locks
 
 void freelock2(void *lock); //for recursive locks
 
+void acquire2(void *lock);
+
 void release2(void *lock); //consumes the lock
 
 void spawn(void* (*f)(void*), void* args);
