atomics/general_atomics.v
@@ -1,4 +1,4 @@
- Require Import VST.veric.rmaps.
+Require Import VST.veric.rmaps.
 Require Import VST.veric.compcert_rmaps.
 Require Import VST.progs.ghosts.
 Require Import VST.progs.conclib.
@@ -6,6 +6,7 @@ Require Import VST.progs.invariants.
 Require Import VST.progs.fupd.
 Require Import VST.floyd.library.
 Require Import VST.floyd.sublist.
+Require Import iris.bi.lib.atomic.
 
 Set Bullet Behavior "Strict Subproofs".
 
@@ -39,6 +40,9 @@ Definition ashift {A B} P (a : A -> mpred) Ei Eo (b : A -> B -> mpred) (Q : B ->
   ((|> P -* |={Eo,Ei}=> (EX x : A, a x *
     ((a x -* |={Ei,Eo}=> |> P) &&
      ALL y : B, b x y -* |={Ei,Eo}=> Q y))))%I.
+
+(* switch to Ralf's? *)
+Locate atomic_update.
 
 Definition atomic_shift {A B} (a : A -> mpred) Ei Eo (b : A -> B -> mpred) (Q : B -> mpred) :=
   EX P : mpred, |> P * (ashift P a Ei Eo b Q && cored).
@@ -1010,6 +1014,39 @@ Notation "'ATOMIC' 'TYPE' W 'OBJ' x 'INVS' Ei Eo 'WITH' x1 : t1 , x2 : t2 , x3 :
    (atomic_spec_nonexpansive_post' W nil _)) (at level 200, x at level 0, Ei at level 0, Eo at level 0,
         x1 at level 0, x2 at level 0, x3 at level 0, x4 at level 0, x5 at level 0, x6 at level 0, x7 at level 0,
              S2 at level 0, r at level 0, T at level 0).
+
+Notation "'ATOMIC' 'TYPE' W 'OBJ' x 'INVS' Ei Eo 'WITH' x1 : t1 , x2 : t2 , x3 : t3 , x4 : t4 , x5 : t5 , x6 : t6 , x7 : t7 'PRE'  [ u , .. , v ] 'PROP' ( Px ; .. ; Py ) 'LOCAL' ( Lx ; .. ; Ly ) 'SEPS' ( S1x ; .. ; S1y ) '|' S2 'POST' [ tz ] 'PROP' () 'LOCAL' ( LQx ; .. ; LQy ) 'SEP' ( SQx ; .. ; SQy )" :=
+  (mk_funspec (pair (cons u%formals .. (cons v%formals nil) ..) tz) cc_default (atomic_spec_type0 W)
+   (fun (ts: list Type) (__a : functors.MixVariantFunctor._functor (dependent_type_functor_rec ts W) mpred * mpred * invG) => let '((x1, x2, x3, x4, x5, x6, x7), Q, inv_names) := __a in
+     PROPx (cons Px%type .. (cons Py%type nil) ..)
+     (LOCALx (cons Lx%type .. (cons Ly%type nil) ..)
+     (SEPx (cons (atomic_shift(B := unit)(inv_names := inv_names) (fun x => S2) Ei Eo (fun x _ => fold_right_sepcon (cons SQx%logic .. (cons SQy%logic nil) ..)) Q) (cons S1x%logic .. (cons S1y%logic nil) ..)))))
+   (fun (ts: list Type) (__a : functors.MixVariantFunctor._functor (dependent_type_functor_rec ts W) mpred * mpred * invG) => let '((x1, x2, x3, x4, x5, x6, x7), Q, inv_names) := __a in
+     PROP () (LOCALx (cons LQx%logic .. (cons LQy%logic nil) ..) (SEP (Q))))
+   (@atomic_spec_nonexpansive_pre0 _ W (cons (fun ts __a => let '(x1, x2, x3, x4, x5, x6, x7) := __a in Px%type) .. (cons (fun ts __a => let '(x1, x2, x3, x4, x5, x6, x7) := __a in Py%type) nil) ..)
+      (cons (fun ts __a => let '(x1, x2, x3, x4, x5, x6, x7) := __a in Lx%type) .. (cons (fun ts __a => let '(x1, x2, x3, x4, x5, x6, x7) := __a in Ly%type) nil) ..)
+      (cons (fun ts __a => let '(x1, x2, x3, x4, x5, x6, x7) := __a in S1x%logic) .. (cons (fun ts __a => let '(x1, x2, x3, x4, x5, x6, x7) := __a in S1y%logic) nil) ..)
+      (fun ts __a x => let '(x1, x2, x3, x4, x5, x6, x7) := __a in S2) Ei Eo
+     (fun ts __a x _ => let '(x1, x2, x3, x4, x5, x6, x7) := __a in fold_right_sepcon (cons SQx%logic .. (cons SQy%logic nil) ..)) _ _ _ _ _)
+   (atomic_spec_nonexpansive_post0 W (cons (fun ts __a _ => let '(x1, x2, x3, x4, x5, x6, x7) := __a in LQx%logic) .. (cons (fun ts __a _ => let '(x1, x2, x3, x4, x5, x6, x7) := __a in LQy%logic) nil) ..) _)) (at level 200, x at level 0, Ei at level 0, Eo at level 0,
+        x1 at level 0, x2 at level 0, x3 at level 0, x4 at level 0, x5 at level 0, x6 at level 0, x7 at level 0,
+             S2 at level 0).
+
+Notation "'ATOMIC' 'TYPE' W 'OBJ' x 'INVS' Ei Eo 'WITH' x1 : t1 , x2 : t2 , x3 : t3 , x4 : t4 , x5 : t5 , x6 : t6 , x7 : t7 'PRE'  [ u , .. , v ] 'PROP' ( Px ; .. ; Py ) 'LOCAL' ( Lx ; .. ; Ly ) 'SEPS' ( S1x ; .. ; S1y ) '|' S2 'POST' [ tz ] 'PROP' () 'LOCAL' () 'SEP' ( SQx ; .. ; SQy )" :=
+  (mk_funspec (pair (cons u%formals .. (cons v%formals nil) ..) tz) cc_default (atomic_spec_type0 W)
+   (fun (ts: list Type) (__a : functors.MixVariantFunctor._functor (dependent_type_functor_rec ts W) mpred * mpred * invG) => let '((x1, x2, x3, x4, x5, x6, x7), Q, inv_names) := __a in
+     PROPx (cons Px%type .. (cons Py%type nil) ..)
+     (LOCALx (cons Lx%type .. (cons Ly%type nil) ..)
+     (SEPx (cons (atomic_shift(B := unit)(inv_names := inv_names) (fun x => S2) Ei Eo (fun x _ => fold_right_sepcon (cons SQx%logic .. (cons SQy%logic nil) ..)) (fun _ => Q)) (cons S1x%logic .. (cons S1y%logic nil) ..)))))
+   (fun (ts: list Type) (__a : functors.MixVariantFunctor._functor (dependent_type_functor_rec ts W) mpred * mpred * invG) => let '((x1, x2, x3, x4, x5, x6, x7), Q, inv_names) := __a in
+     PROP () LOCAL () (SEP (Q)))
+   (@atomic_spec_nonexpansive_pre0 _ W (cons (fun ts __a => let '(x1, x2, x3, x4, x5, x6, x7) := __a in Px%type) .. (cons (fun ts __a => let '(x1, x2, x3, x4, x5, x6, x7) := __a in Py%type) nil) ..)
+      (cons (fun ts __a => let '(x1, x2, x3, x4, x5, x6, x7) := __a in Lx%type) .. (cons (fun ts __a => let '(x1, x2, x3, x4, x5, x6, x7) := __a in Ly%type) nil) ..)
+      (cons (fun ts __a => let '(x1, x2, x3, x4, x5, x6, x7) := __a in S1x%logic) .. (cons (fun ts __a => let '(x1, x2, x3, x4, x5, x6, x7) := __a in S1y%logic) nil) ..)
+      (fun ts __a x => let '(x1, x2, x3, x4, x5, x6, x7) := __a in S2) Ei Eo
+     (fun ts __a x _ => let '(x1, x2, x3, x4, x5, x6, x7) := __a in fold_right_sepcon (cons SQx%logic .. (cons SQy%logic nil) ..)) _ _ _ _ _)
+   (atomic_spec_nonexpansive_post0 W nil _)) (at level 200, x at level 0, Ei at level 0, Eo at level 0,
+        x1 at level 0, x2 at level 0, x3 at level 0, x4 at level 0, x5 at level 0, x6 at level 0, x7 at level 0, S2 at level 0).
 
 Notation "'ATOMIC' 'TYPE' W 'OBJ' x 'INVS' Ei Eo 'WITH' x1 : t1 , x2 : t2 , x3 : t3 , x4 : t4 , x5 : t5 , x6 : t6 , x7 : t7 , x8 : t8 'PRE'  [ u , .. , v ] 'PROP' ( Px ; .. ; Py ) 'LOCAL' ( Lx ; .. ; Ly ) 'SEPS' ( S1x ; .. ; S1y ) '|' S2 'POST' [ tz ] 'EX' r : T , 'PROP' () 'LOCAL' ( LQx ; .. ; LQy ) 'SEP' ( SQx ; .. ; SQy )" :=
   (mk_funspec (pair (cons u%formals .. (cons v%formals nil) ..) tz) cc_default (atomic_spec_type W T)
